test out high order predicate

concurrency/disciplined/sharedexclusive-linearatomic/ShardedHashTable.i.dfy
@@ -76,43 +76,6 @@ module ShardedHashTable refines ShardedStateMachine {
     unit().(stubs := multiset{Stub(id, output)})
   }
 
-  // function oneRowTable(k: nat, entry: Entry) : Table
-  // requires 0 <= k < FixedSize()
-  // {
-  //   seq(FixedSize(), i => if i == k then Some(entry) else None)
-  // }
-
-  // function oneRowResource(k: nat, entry: Entry, cap: nat) : Variables 
-  // requires 0 <= k < FixedSize()
-  // {
-  //   Variables(oneRowTable(k, entry), Count.Variables(cap), multiset{}, multiset{})
-  // }
-
-  // function twoRowsTable(k1: nat, entry1: Entry, k2: nat, entry2: Entry) : Table
-  // requires 0 <= k1 < FixedSize()
-  // requires 0 <= k2 < FixedSize()
-  // requires k1 != k2
-  // {
-  //   seq(FixedSize(), i => if i == k1 then Some(entry1) else if i == k2 then Some(entry2) else None)
-  // }
-
-  // function twoRowsResource(k1: nat, entry1: Entry, k2: nat, entry2: Entry, cap: nat) : Variables 
-  // requires 0 <= k1 < FixedSize()
-  // requires 0 <= k2 < FixedSize()
-  // requires k1 != k2
-  // {
-  //   Variables(twoRowsTable(k1, entry1, k2, entry2), Count.Variables(cap), multiset{}, multiset{})
-  // }
-
-  predicate IsInputResource(in_r: Variables, rid: int, input: Ifc.Input)
-  {
-    && in_r.Variables?
-    && in_r.table == unitTable()
-    && in_r.insert_capacity.value == 0
-    && in_r.tickets == multiset { Ticket(rid, input) }
-    && in_r.stubs == multiset { }
-  }
-
   predicate nonoverlapping<A>(a: seq<Option<A>>, b: seq<Option<A>>)
   requires |a| == FixedSize()
   requires |b| == FixedSize()
@@ -168,7 +131,6 @@ module ShardedHashTable refines ShardedStateMachine {
       assert add(x, add(y, z)) == add(add(x, y), z);
     }
   }
-
   predicate Init(s: Variables)
   {
     && s.Variables?
@@ -178,23 +140,36 @@ module ShardedHashTable refines ShardedStateMachine {
     && s.stubs == multiset{}
   }
 
+  predicate IsInputResource(in_r: Variables, rid: int, input: Ifc.Input)
+  {
+    && in_r.Variables?
+    && in_r.table == unitTable()
+    && in_r.insert_capacity.value == 0
+    && in_r.tickets == multiset { Ticket(rid, input) }
+    && in_r.stubs == multiset { }
+  }
+
 //////////////////////////////////////////////////////////////////////////////
 // Transition definitions
 //////////////////////////////////////////////////////////////////////////////
 
-  datatype InsertStutter = InsertStutter(key: Key, val: Value, start: Index, end: Index)
-
   datatype Step =
-    | InsertStep(ticket: Ticket, stutters: seq<InsertStutter>)
-    | OverwriteStep(ticket: Ticket, stutter: InsertStutter)
+    | InsertStep(ticket: Ticket, start: Index, end: Index)
+    | OverwriteStep(ticket: Ticket, i: Index)
 
     | QueryFoundStep(ticket: Ticket, i: Index)
     | QueryNotFoundStep(ticket: Ticket, end: Index)
 
-    | RemoveStep(ticket: Ticket, i: Index, end: Index)
+    | RemoveStep(ticket: Ticket, start: Index, end: Index)
     | RemoveNotFoundStep(ticket: Ticket, end: Index)
 
 // Insert transition definitions
+
+  // unwrapped_index
+  function adjust2(i: Index, root: Index) : int
+  {
+    if i <= root then FixedSize() + i else i
+  }
 
   // insert_h: hash of the key we are trying to insert
   // slot_h : hash of the key at slot_index
@@ -206,7 +181,23 @@ module ShardedHashTable refines ShardedStateMachine {
     || slot_idx < search_h < slot_h// search_h, slot_h wrap around the end of array
   }
 
-  predicate ShouldSkipSlot(table: FixedTable, insert_key: Key, slot_index: Index)
+  predicate TrueForSubTableNoWrap(table: FixedTable, start: Index, end: int, key: Key, p: (FixedTable, Index, Key) -> bool)
+    requires start <= end <= FixedSize();
+  {
+    forall i | start <= i < end :: p(table, i, key)
+  }
+
+  predicate TrueForSubTable(table: FixedTable, start: Index, end: Index, key: Key, p: (FixedTable, Index, Key) -> bool)
+  {
+    (if start <= end then
+      TrueForSubTableNoWrap(table, start, end, key, p)
+    else (
+      && TrueForSubTableNoWrap(table, start, FixedSize(), key, p)
+      && TrueForSubTableNoWrap(table, 0, end, key, p)
+    ))
+  }
+
+  predicate ShouldSkipSlot(table: FixedTable, slot_index: Index, insert_key: Key)
   {
     && table[slot_index].Some?
     && table[slot_index].value.Full?
@@ -215,249 +206,210 @@ module ShardedHashTable refines ShardedStateMachine {
     !ShouldHashGoBefore(insert_h, slot_h, slot_index)
   }
 
-
-  predicate ShouldSkipSlotsNoWrap(table: FixedTable, insert_key: Key, start: Index, end: int)
-    requires start <= end <= FixedSize();
+  predicate ShouldSkipSlots(table: FixedTable, start: Index, end: Index, key: Key )
   {
-    forall i | start <= i < end :: ShouldSkipSlot(table, insert_key, i)
+    TrueForSubTable(table, start, end, key, ShouldSkipSlot)
   }
 
-  predicate ShouldSkipSlots(table: FixedTable, stutter: InsertStutter)
+  predicate KeyNotInSlot(table: FixedTable, slot_index: Index, key: Key)
   {
-    var InsertStutter(insert_key, _, start, end) := stutter;
-    && table[end].Some?
-    && (if start <= end then
-      ShouldSkipSlotsNoWrap(table, insert_key, start, end)
-    else (
-      && ShouldSkipSlotsNoWrap(table, insert_key, start, FixedSize())
-      && ShouldSkipSlotsNoWrap(table, insert_key, 0, end)
-    ))
+    && table[slot_index].Some?
+    && table[slot_index].value.Full?
+    && table[slot_index].value.key != key
   }
 
-  predicate TableInsertSwapEnable(table: FixedTable, stutter: InsertStutter)
+  predicate KeyNotFound(table: FixedTable, start: Index, end: Index, key: Key)
   {
-    var InsertStutter(insert_key, _, _, end) := stutter;
-    // we should skip these
-    && ShouldSkipSlots(table, stutter)
-    // the entry at end index should be swapped out
-    && table[end].value.Full?
-    && table[end].value.key != insert_key
-    && !ShouldSkipSlot(table, insert_key, end)
+    TrueForSubTable(table, start, end, key, KeyNotInSlot)
   }
-
-  predicate TableInsertDoneEnable(table: FixedTable, stutter: InsertStutter)
-  {
-    // we should skip these
-    && ShouldSkipSlots(table, stutter)
-    // the entry at end index is empty
-    && table[stutter.end].value.Empty?
-  }
-
-  predicate TableOverwriteEnable(table: FixedTable, stutter: InsertStutter)
-  {
-    var InsertStutter(insert_key, _, _, end) := stutter;
-    // we should skip these, TODO: we might not need this?
-    && ShouldSkipSlots(table, stutter) 
-    // the entry at end index has the same key
-    && table[end].value.Full?
-    && table[end].value.key == insert_key
-  }
-
-  function TableInsert(table: FixedTable, stutter: InsertStutter) : FixedTable
-    requires 
-      || TableInsertSwapEnable(table, stutter)
-      || TableInsertDoneEnable(table, stutter)
-      || TableOverwriteEnable(table, stutter)
-  {
-    var InsertStutter(key, val, _, end) := stutter;
-    table[end := Some(Full(key, val))]
-  }
-
-  predicate TableInsertEnableRec(table: FixedTable, stutters: seq<InsertStutter>)
-    requires |stutters| >= 1
-    decreases |stutters|
-  {
-    var curr := stutters[0];
-    if |stutters| == 1 then
-        TableInsertDoneEnable(table, curr)
-    else
-      (
-        // next starts at current end
-        && curr.end == stutters[1].start
-        && TableInsertSwapEnable(table, curr)
-        && var table' := TableInsert(table, curr);
-        // recurse on the rest of the steps
-        && TableInsertEnableRec(table', stutters[1..])
-      )
-  }
-
-  function TableInsertRec(table: FixedTable, stutters: seq<InsertStutter>): FixedTable
-    requires |stutters| >= 1
-    requires TableInsertEnableRec(table, stutters)
-    decreases |stutters|
-  {
-    var curr := stutters[0];
-    if |stutters| == 1 then
-      TableInsert(table, curr)
-    else
-      var table' := TableInsert(table, curr);
-      TableInsertRec(table', stutters[1..])
-  }
-
-  predicate Insert(v: Variables, v': Variables, ticket: Ticket, stutters: seq<InsertStutter>)
-  {
-    && v.Variables?
-    && ticket in v.tickets
-    && ticket.input.InsertInput?
-    && v.insert_capacity.value >= 1
-
-    && |stutters| >= 1
-    // the first step starts at the insert key hash
-    && var first := stutters[0];
-    && first.start == hash(first.key)
-    && first.key == ticket.input.key
-
-    && TableInsertEnableRec(v.table, stutters)
-
-    && v' == v
-      .(tickets := v.tickets - multiset{ticket})
-      .(stubs := v.stubs + multiset{Stub(ticket.rid, MapIfc.InsertOutput(true))})
-      .(insert_capacity := Count.Variables(v.insert_capacity.value - 1))
-      .(table := TableInsertRec(v.table, stutters))
-  }
-
-  predicate Overwrite(v: Variables, v': Variables, ticket: Ticket, stutter: InsertStutter)
-  {
-    && v.Variables?
-    && ticket in v.tickets
-    && ticket.input.InsertInput?
-
-    && TableOverwriteEnable(v.table, stutter)
-
-    && v' == v
-      .(tickets := v.tickets - multiset{ticket})
-      .(stubs := v.stubs + multiset{Stub(ticket.rid, MapIfc.InsertOutput(true))})
-      .(table := TableInsert(v.table, stutter))
-  }
-
-// Query transition definitions
-
-  predicate QueryFound(v: Variables, v': Variables, ticket: Ticket, i: Index)
-  {
-    && v.Variables?
-    && v'.Variables?
-    && ticket in v.tickets
-    && ticket.input.QueryInput?
-    && v.table[i].Some?
-    && v.table[i].value.Full?
-    && v.table[i].value.key == ticket.input.key
-    && v' == v
-      .(tickets := v.tickets - multiset{ticket})
-      .(stubs := v.stubs + multiset{
-        Stub(ticket.rid, MapIfc.QueryOutput(Found(v.table[i].value.value)))})
-  }
-
-  predicate KeyNotFound(table: FixedTable, key: Key, end: Index)
-  {
-    && table[end].Some?
-    && table[end].value.Empty?
-    && var h := hash(key) as int;
-    && (h <= end ==> forall j | h <= j < end     :: table[j].Some? && table[j].value.Full? && table[j].value.key != key)
-    && (h > end  ==> forall j | h <= j < |table| :: table[j].Some? && table[j].value.Full? && table[j].value.key != key)
-    && (h > end  ==> forall j | 0 <= j < end     :: table[j].Some? && table[j].value.Full? && table[j].value.key != key)
-  }
-
-  predicate QueryNotFound(v: Variables, v': Variables, ticket: Ticket, end: Index)
-  {
-    && v.Variables?
-    && v'.Variables?
-    && ticket in v.tickets
-    && ticket.input.QueryInput?
-    && KeyNotFound(v.table, ticket.input.key, end)
-    && v' == v
-      .(tickets := v.tickets - multiset{ticket})
-      .(stubs := v.stubs + multiset{Stub(ticket.rid, MapIfc.QueryOutput(NotFound))})
-  }
-
-// Remove transition definitions
-
-  predicate RemoveNotFound(v: Variables, v': Variables, ticket: Ticket, end: Index)
-  {
-    && v.Variables?
-    && v'.Variables?
-    && ticket in v.tickets
-    && ticket.input.RemoveInput?
-    && KeyNotFound(v.table, ticket.input.key, end)
-    && v' == v
-      .(tickets := v.tickets - multiset{ticket})
-      .(stubs := v.stubs + multiset{Stub(ticket.rid, MapIfc.RemoveOutput(false))})
-  }
-
-  predicate LeftShift_PartialState(table: Table, table': Table, shift: LeftShift)
-  {
-    && 0 <= shift.start < |table|
-    && 0 <= shift.end < |table|
-    && |table'| == |table|
-
-    && (shift.start <= shift.end ==>
-      && (forall i | 0 <= i < shift.start :: table'[i] == table[i]) // untouched things
-      && (forall i | shift.start <= i < shift.end :: table'[i] == table[i+1] && table'[i].Some?) // touched things
-      && table'[shift.end] == Some(Empty) // the end should be empty
-      && (forall i | shift.end < i < |table'| :: table'[i] == table[i]) // untouched things
-    )
-
-    && (shift.start > shift.end ==>
-      && (forall i | 0 <= i < shift.end :: table'[i] == table[i+1]) // shift second half 
-      && table'[shift.end] == Some(Empty) // the end should be empty 
-      && (forall i | shift.end < i < shift.start :: table'[i] == table[i]) // untouched things
-      && (forall i | shift.start <= i < |table'| - 1 :: table'[i] == table[i+1] && table'[i].Some?) // shift first half 
-      && table'[ |table'| - 1 ] == table[0] // shift around the wrap 
-    )
-  }
-
-  predicate Remove(v: Variables, v': Variables, ticket: Ticket, i: int, end: int)
-  {
-    && v.Variables?
-    && v'.Variables?
-    && ticket in v.tickets
-    && ticket.input.RemoveInput?
-    && 0 <= i < |v.table|
-    && v.table[i].Some?
-    && v.table[i].value.Full?
-    && v.table[i].value.key == ticket.input.key
-    && LeftShift_PartialState(v.table, v'.table, LeftShift(i, end))
-    && v' == v.(table := v'.table)
-        .(tickets := v.tickets - multiset{ticket})
-        .(stubs := v.stubs + multiset{Stub(ticket.rid, MapIfc.RemoveOutput(true))})
-  }
-
-// All transitions
-
-  predicate NextStep(v: Variables, v': Variables, step: Step)
-  {
-    match step {
-      case InsertStep(ticket, stutters) => Insert(v, v', ticket, stutters)
-      case OverwriteStep(ticket, stutter) => Overwrite(v, v', ticket, stutter)
-      case QueryFoundStep(ticket, i) => QueryFound(v, v', ticket, i)
-      case QueryNotFoundStep(ticket, end) => QueryNotFound(v, v', ticket, end)
-      case RemoveStep(ticket, i, end) => Remove(v, v', ticket, i, end)
-      case RemoveNotFoundStep(ticket, end) => RemoveNotFound(v, v', ticket, end)
-    }
-  }
-
-  predicate Next(s: Variables, s': Variables)
-  {
-    exists step :: NextStep(s, s', step)
-  }
-
-//////////////////////////////////////////////////////////////////////////////
-// global-level Invariant proof
-//////////////////////////////////////////////////////////////////////////////
 
   predicate Complete(table: FixedTable)
   {
     && (forall i: Index :: table[i].Some?)
   }
+
+  predicate TableRightShift(table: FixedTable, table': FixedTable, inserted: Option<Entry>, start: Index, end: Index)
+  {
+    && (start <= end ==>
+      && (forall i | 0 <= i < start :: table'[i] == table[i])
+      && table'[start] == inserted
+      && (forall i | start < i <= end :: table'[i] == table[i-1])
+      && (forall i | end < i < |table'| :: table'[i] == table[i])
+    )
+    && (start > end ==>
+      && table'[0] == table[ |table| - 1]
+      && (forall i | 0 < i <= end :: table'[i] == table[i-1])
+      && (forall i | end < i < start :: table'[i] == table[i])
+      && table'[start] == inserted
+      && (forall i | start < i < |table'| :: table'[i] == table[i-1])
+    )
+  }
+
+  function TableRightShiftTransition(table: FixedTable, inserted: Option<Entry>, start: Index, end: Index) : (table': FixedTable)
+    ensures TableRightShift(table, table', inserted, start, end)
+  {
+    if start == end then
+      table[start := inserted]
+    else if start < end then
+      table[..start] + [inserted] + table[start..end] + table[end+1..]
+    else
+      var last_index := |table| - 1;
+      [table[last_index]] + table[..end] + table[end+1..start] + [inserted] + table[start..last_index]
+  }
+
+  predicate Insert(v: Variables, v': Variables, ticket: Ticket, kv: (Key, Value), start: Index, end: Index)
+  {
+    var (key, value) := kv;
+    var h := hash(key);
+    && v.Variables?
+    && var table := v.table;
+    && ticket in v.tickets
+    && ticket.input.InsertInput?
+    && v.insert_capacity.value >= 1
+
+    // skip upto (not including) start
+    && ShouldSkipSlots(table, h, start, key)
+    // insert at start
+    && !ShouldSkipSlot(table, start, key)
+    // end is empty 
+    && table[end].Some?
+    && table[end].value.Empty?
+
+    && KeyNotFound(table, start, end, key)
+
+    && v'.Variables?
+    && TableRightShift(v.table, v'.table, Some(Full(key, value)), start, end)
+  }
+
+//   predicate TableLeftShift(table: FixedTable, table': FixedTable, start: Index, end: Index)
+//   {
+//     && (start <= end ==>
+//       && (forall i | 0 <= i < start :: table'[i] == table[i]) 
+//       // shifted entries
+//       && (forall i | start <= i < end :: table'[i] == table[i+1] && table'[i].Some?) 
+//       && table'[end] == Some(Empty) 
+//       && (forall i | end < i < |table'| :: table'[i] == table[i]) // untouched things
+//     )
+//     && (start > end ==>
+//       && (forall i | 0 <= i < end :: table'[i] == table[i+1]) // shift second half 
+//       && table'[end] == Some(Empty) // the end should be empty 
+//       && (forall i | end < i < start :: table'[i] == table[i]) // untouched things
+//       && (forall i | start <= i < |table'| - 1 :: table'[i] == table[i+1] && table'[i].Some?) // shift first half 
+//       && table'[ |table'| - 1 ] == table[0] // shift around the wrap 
+//     )
+//   }
+
+//   predicate TableOverwriteEnable(table: FixedTable, key: Key, end: Index)
+//   {
+//     // the entry at end index has the same key
+//     && table[end].Some?
+//     && table[end].value.Full?
+//     && table[end].value.key == key
+//   }
+
+//   predicate Overwrite(v: Variables, v': Variables, ticket: Ticket, kv: (Key, Value), end: Index)
+//   {
+//     var (key, value) := kv;
+//     && v.Variables?
+//     && ticket in v.tickets
+//     && ticket.input.InsertInput?
+
+//     && TableOverwriteEnable(v.table, key, end)
+
+//     && v' == v
+//       .(tickets := v.tickets - multiset{ticket})
+//       .(stubs := v.stubs + multiset{Stub(ticket.rid, MapIfc.InsertOutput(true))})
+//       .(table := v.table[end := Some(Full(key, value))])
+//   }
+
+// // Query transition definitions
+
+//   predicate QueryFound(v: Variables, v': Variables, ticket: Ticket, i: Index)
+//   {
+//     && v.Variables?
+//     && v'.Variables?
+//     && ticket in v.tickets
+//     && ticket.input.QueryInput?
+//     && v.table[i].Some?
+//     && v.table[i].value.Full?
+//     && v.table[i].value.key == ticket.input.key
+//     && v' == v
+//       .(tickets := v.tickets - multiset{ticket})
+//       .(stubs := v.stubs + multiset{
+//         Stub(ticket.rid, MapIfc.QueryOutput(Found(v.table[i].value.value)))})
+//   }
+
+//   predicate QueryNotFound(v: Variables, v': Variables, ticket: Ticket, end: Index)
+//   {
+//     && v.Variables?
+//     && v'.Variables?
+//     && ticket in v.tickets
+//     && ticket.input.QueryInput?
+
+//     && v.table[end].Some?
+//     && v.table[end].value.Empty?
+
+//     && KeyNotFound(v.table, ticket.input.key, hash(ticket.input.key), end)
+//     && v' == v
+//       .(tickets := v.tickets - multiset{ticket})
+//       .(stubs := v.stubs + multiset{Stub(ticket.rid, MapIfc.QueryOutput(NotFound))})
+//   }
+
+// // Remove transition definitions
+
+//   predicate RemoveNotFound(v: Variables, v': Variables, ticket: Ticket, end: Index)
+//   {
+//     && v.Variables?
+//     && v'.Variables?
+//     && ticket in v.tickets
+//     && ticket.input.RemoveInput?
+
+//     && v.table[end].Some?
+//     && v.table[end].value.Empty?
+
+//     && KeyNotFound(v.table, ticket.input.key, hash(ticket.input.key), end)
+//     && v' == v
+//       .(tickets := v.tickets - multiset{ticket})
+//       .(stubs := v.stubs + multiset{Stub(ticket.rid, MapIfc.RemoveOutput(false))})
+//   }
+
+//   predicate Remove(v: Variables, v': Variables, ticket: Ticket, start: Index, end: Index)
+//   {
+//     && v.Variables?
+//     && v'.Variables?
+//     && ticket in v.tickets
+//     && ticket.input.RemoveInput?
+//     && v.table[start].Some?
+//     && v.table[start].value.Full?
+//     && v.table[start].value.key == ticket.input.key
+//     && TableLeftShift(v.table, v'.table, start, end)
+//     && v' == v.(table := v'.table)
+//         .(tickets := v.tickets - multiset{ticket})
+//         .(stubs := v.stubs + multiset{Stub(ticket.rid, MapIfc.RemoveOutput(true))})
+//   }
+
+// // All transitions
+
+//   // predicate NextStep(v: Variables, v': Variables, step: Step)
+//   // {
+//   //   match step {
+//   //     case InsertStep(ticket, stutters) => Insert(v, v', ticket, stutters)
+//   //     case OverwriteStep(ticket, stutter) => Overwrite(v, v', ticket, stutter)
+//   //     case QueryFoundStep(ticket, i) => QueryFound(v, v', ticket, i)
+//   //     case QueryNotFoundStep(ticket, end) => QueryNotFound(v, v', ticket, end)
+//   //     case RemoveStep(ticket, i, end) => Remove(v, v', ticket, i, end)
+//   //     case RemoveNotFoundStep(ticket, end) => RemoveNotFound(v, v', ticket, end)
+//   //   }
+//   // }
+
+//   // predicate Next(s: Variables, s': Variables)
+//   // {
+//   //   exists step :: NextStep(s, s', step)
+//   // }
+
+// //////////////////////////////////////////////////////////////////////////////
+// // global-level Invariant proof
+// //////////////////////////////////////////////////////////////////////////////
 
   // Keys are unique, although we don't count entries being removed
   predicate KeysUnique(table: FixedTable)
@@ -470,31 +422,15 @@ module ShardedHashTable refines ShardedStateMachine {
       :: table[i].value.key != table[j].value.key
   }
 
-  // function adjust(i: Index, root: int) : int
-  //   requires 0 <= root <= FixedSize()
-  // {
-  //   if i < root then FixedSize() + i else i
-  // }
-
-  // unwrapped_index
-  function adjust2(i: Index, root: Index) : int
-  {
-    if i <= root then FixedSize() + i else i
-  }
-
-  // lemma test(i: Index, e: Index)
-  // {
-  //   assert adjust2(i, e) == adjust(i, e +1);
-  // }
-
-  predicate ValidHashInIndex(table: FixedTable, e: Index, i: Index)
+  predicate ValidHashInSlot(table: FixedTable, e: Index, i: Index)
     requires Complete(table)
   {
     // No matter which empty pivot cell 'e' we choose, every entry is 'downstream'
     // of the place that it hashes to.
     // Likewise for insert pointers and others
 
-    table[e].value.Empty? && table[i].value.Full? ==>
+    (table[e].value.Empty? && table[i].value.Full?)
+      ==>
     (
       var h := hash(table[i].value.key);
       adjust2(h, e) <= adjust2(i, e)
@@ -526,7 +462,7 @@ module ShardedHashTable refines ShardedStateMachine {
   {
     && Complete(table)
     && KeysUnique(table)
-    && (forall e: Index, i: Index :: ValidHashInIndex(table, e, i))
+    && (forall e: Index, i: Index :: ValidHashInSlot(table, e, i))
     && (forall e: Index, j: Index, k: Index :: ValidHashOrdering(table, e, j, k))
   }
 
@@ -556,9 +492,9 @@ module ShardedHashTable refines ShardedStateMachine {
     && TableQuantityInv(s)
   }
 
-//////////////////////////////////////////////////////////////////////////////
-// Proof that Init && Next maintains Inv
-//////////////////////////////////////////////////////////////////////////////
+// //////////////////////////////////////////////////////////////////////////////
+// // Proof that Init && Next maintains Inv
+// //////////////////////////////////////////////////////////////////////////////
 
   lemma TableQuantityReplace1(t: Table, t': Table, i: Index)
     requires 0 <= i < |t| == |t'|
@@ -574,212 +510,197 @@ module ShardedHashTable refines ShardedStateMachine {
     }
   }
 
-  lemma TableInsertSwapPreservesInv(s: Variables, s': Variables, stutter: InsertStutter)
-    requires Inv(s);
-    requires s'.Variables?
-    requires TableInsertSwapEnable(s.table, stutter)
-    requires TableInsert(s.table, stutter) == s'.table;
-  {
-    var end := stutter.end;
+  // lemma OverwriteStepPreservesInv(s: Variables, s': Variables, ticket: Ticket, kv: (Key, Value), end: Index)
+  //   requires Inv(s)
+  //   requires Overwrite(s, s', ticket, kv, end)
+  //   ensures Inv(s')
+  // {
+  //   assert forall i: Index :: s'.table[i].value.Full? ==> 
+  //     s'.table[i].value.key == s.table[i].value.key;
+    
+  //   forall e: Index, i: Index
+  //     ensures ValidHashInSlot(s'.table, e, i)
+  //   {
+  //     assert ValidHashInSlot(s.table, e, i);
+  //   }
 
+  //   forall e: Index, j: Index, k: Index
+  //     ensures ValidHashOrdering(s'.table, e, j, k)
+  //   {
+  //     assert ValidHashOrdering(s.table, e, j, k);
+  //     assert ValidHashInSlot(s.table, e, j);
+  //     assert ValidHashInSlot(s.table, e, k);
+  //   }
+
+  //   TableQuantityReplace1(s.table, s'.table, end);
+  // }
+
+  lemma InsertStepPreservesInv(s: Variables, s': Variables, ticket: Ticket, kv: (Key, Value), start: Index, end: Index)
+    requires Inv(s)
+    requires Insert(s, s', ticket, kv, start, end)
+  {
+    var (key, value) := kv;
     var table := s.table;
     var table' := s'.table;
 
-    assert forall i: Index ::
-      table'[i].value.Full? && i != end ==> 
-      table'[i].value.key == table[i].value.key;
+    assert table' == TableRightShiftTransition(table, Some(Full(key, value)), start, end);
 
-    forall e: Index, i: Index
-      ensures ValidHashInIndex(table', e, i)
+    forall i: Index, j: Index |
+        && i != j
+        && table'[i].value.Full?
+        && table'[j].value.Full?
+    ensures table'[i].value.key != table'[j].value.key
     {
-      assert ValidHashInIndex(table, e, i);
-      assume false;
-      // var i' := if i > 0 then i - 1 else |table| - 1;
-      // assert ValidHashInIndex(s.table, e, i');
-    }
+      if start == end {
+        assert ValidHashInSlot(table, end, start);
 
-    forall e: Index, j: Index, k: Index
-      ensures ValidHashOrdering(table', e, j, k)
-    {
-      if j != end && k != end {
-        assert ValidHashOrdering(table, e, j, k);
-        assert ValidHashInIndex(table, e, j);
-        assert ValidHashInIndex(table, e, k);
-      } else if j == end && k != end {
-        if table[e].value.Empty?
-          && table[k].value.Full?
-          && adjust2(j, e) < adjust2(k, e) {
-
-          assert ValidHashOrdering(table, e, j, k);
-          assert ValidHashInIndex(table, e, j);
-          assert ValidHashInIndex(table, e, k);
-          assert ValidHashInIndex(table', e, j);
-
-          var hj := hash(table[j].value.key);
-          var hj' := hash(table'[j].value.key);
-          var hk := hash(table[k].value.key);
-
-          assert ShouldHashGoBefore(hj', hj, j);
-
-          if adjust2(hj, e) <= adjust2(hk, e) < adjust2(j, e) < adjust2(k, e) {
-            assert adjust2(hj', e) <= adjust2(hj, e);
-          }
-        } 
-      } else if j != end && k == end {
+        assume false;
+      } else {
         assume false;
       }
     }
+
+    // assert KeysUnique(s'.table);
+
+    // forall e: Index, i: Index
+    //   ensures ValidHashInSlot(s'.table, e, i)
+    // {
+
+    //   assert ValidHashInSlot(s.table, e, i);
+    // }
+
+    // forall e: Index, j: Index, k: Index
+    //   ensures ValidHashOrdering(s'.table, e, j, k)
+    // {
+    //   assert ValidHashOrdering(s.table, e, j, k);
+    //   assert ValidHashInSlot(s.table, e, j);
+    //   assert ValidHashInSlot(s.table, e, k);
+    // }
   }
 
-  lemma OverwriteStepPreservesInv(s: Variables, s': Variables, ticket: Ticket, stutter: InsertStutter)
-    requires Inv(s)
-    requires Overwrite(s, s', ticket, stutter)
-    ensures Inv(s')
-  {
-    assert forall i: Index :: s'.table[i].value.Full? ==> 
-      s'.table[i].value.key == s.table[i].value.key;
-    
-    forall e: Index, i: Index
-      ensures ValidHashInIndex(s'.table, e, i)
-    {
-      assert ValidHashInIndex(s.table, e, i);
-    }
+//   lemma RemoveStepPreservesInv(s: Variables, s': Variables, ticket: Ticket, i: Index, end: Index)
+//     requires Inv(s)
+//     requires Remove(s, s',ticket, i, end)
+//     ensures Inv(s')
+//   {
+//     assume false;
+//   }
 
-    forall e: Index, j: Index, k: Index
-      ensures ValidHashOrdering(s'.table, e, j, k)
-    {
-      assert ValidHashOrdering(s.table, e, j, k);
-      assert ValidHashInIndex(s.table, e, j);
-      assert ValidHashInIndex(s.table, e, k);
-    }
+//   lemma NextStepPreservesInv(s: Variables, s': Variables, step: Step)
+//   requires Inv(s)
+//   requires NextStep(s, s', step)
+//   ensures Inv(s')
+//   {
+//     match step {
+//       case InsertStep(ticket, stutters) => assume false;
+//       case OverwriteStep(ticket, stutter) => 
+//         OverwriteStepPreservesInv(s, s', ticket, stutter);
+//       case RemoveStep(ticket, i, end) =>
+//         RemoveStepPreservesInv(s, s', ticket, i, end);
+//       case _ => assert Inv(s');
+//     }
+//   }
 
-    TableQuantityReplace1(s.table, s'.table, stutter.end);
-  }
+//   lemma Next_PreservesInv(s: Variables, s': Variables)
+//   requires Inv(s)
+//   requires Next(s, s')
+//   ensures Inv(s')
+//   {
+//     var step :| NextStep(s, s', step);
+//     NextStep_PreservesInv(s, s', step);
+//   }
 
-  lemma RemoveStepPreservesInv(s: Variables, s': Variables, ticket: Ticket, i: Index, end: Index)
-    requires Inv(s)
-    requires Remove(s, s',ticket, i, end)
-    ensures Inv(s')
-  {
-    assume false;
-  }
+// //////////////////////////////////////////////////////////////////////////////
+// // fragment-level validity defined wrt Inv
+// //////////////////////////////////////////////////////////////////////////////
+//   predicate Valid(s: Variables)
+//     ensures Valid(s) ==> s.Variables?
+//   {
+//     && s.Variables?
+//     && exists t :: Inv(add(s, t))
+//   }
 
-  lemma NextStepPreservesInv(s: Variables, s': Variables, step: Step)
-  requires Inv(s)
-  requires NextStep(s, s', step)
-  ensures Inv(s')
-  {
-    match step {
-      case InsertStep(ticket, stutters) => assume false;
-      case OverwriteStep(ticket, stutter) => 
-        OverwriteStepPreservesInv(s, s', ticket, stutter);
-      case RemoveStep(ticket, i, end) =>
-        RemoveStepPreservesInv(s, s', ticket, i, end);
-      case _ => assert Inv(s');
-    }
-  }
-/*
+//   lemma InvImpliesValid(s: Variables)
+//     requires Inv(s)
+//     ensures Valid(s)
+//   {
+//     // reveal Valid();
+//     add_unit(s);
+//   }
 
-  lemma Next_PreservesInv(s: Variables, s': Variables)
-  requires Inv(s)
-  requires Next(s, s')
-  ensures Inv(s')
-  {
-    var step :| NextStep(s, s', step);
-    NextStep_PreservesInv(s, s', step);
-  }
+//   lemma EmptyTableQuantityIsZero(infos: Table)
+//     requires (forall i | 0 <= i < |infos| :: infos[i] == Some(Empty))
+//     ensures TableQuantity(infos) == 0
+//   {
+//     reveal_TableQuantity();
+//   }
 
-//////////////////////////////////////////////////////////////////////////////
-// fragment-level validity defined wrt Inv
-//////////////////////////////////////////////////////////////////////////////
-  predicate Valid(s: Variables)
-    ensures Valid(s) ==> s.Variables?
-  {
-    && s.Variables?
-    && exists t :: Inv(add(s, t))
-  }
+//   lemma InitImpliesValid(s: Variables)
+//   //requires Init(s)
+//   //ensures Valid(s)
+//   {
+//     EmptyTableQuantityIsZero(s.table);
+//     InvImpliesValid(s);
+//   }
 
-  lemma InvImpliesValid(s: Variables)
-    requires Inv(s)
-    ensures Valid(s)
-  {
-    // reveal Valid();
-    add_unit(s);
-  }
+//   lemma NextPreservesValid(s: Variables, s': Variables)
+//   //requires Next(s, s')
+//   //requires Valid(s)
+//   ensures Valid(s')
+//   {
+//     // reveal Valid();
+//     var t :| Inv(add(s, t));
+//     InvImpliesValid(add(s, t));
+//     update_monotonic(s, s', t);
+//     Next_PreservesInv(add(s, t), add(s', t));
+//   }
 
-  lemma EmptyTableQuantityIsZero(infos: Table)
-    requires (forall i | 0 <= i < |infos| :: infos[i] == Some(Empty))
-    ensures TableQuantity(infos) == 0
-  {
-    reveal_TableQuantity();
-  }
+//   predicate TransitionEnable(s: Variables, step: Step)
+//   {
+//     match step {
+//     }
+//   }
 
-  lemma InitImpliesValid(s: Variables)
-  //requires Init(s)
-  //ensures Valid(s)
-  {
-    EmptyTableQuantityIsZero(s.table);
-    InvImpliesValid(s);
-  }
+//   function GetTransition(s: Variables, step: Step): (s': Variables)
+//     requires TransitionEnable(s, step)
+//     ensures NextStep(s, s', step);
+//   {
+//     match step {
+//     }
+//   }
 
-  lemma NextPreservesValid(s: Variables, s': Variables)
-  //requires Next(s, s')
-  //requires Valid(s)
-  ensures Valid(s')
-  {
-    // reveal Valid();
-    var t :| Inv(add(s, t));
-    InvImpliesValid(add(s, t));
-    update_monotonic(s, s', t);
-    Next_PreservesInv(add(s, t), add(s', t));
-  }
+//   // Reduce boilerplate by letting caller provide explicit step, which triggers a quantifier for generic Next()
+//   glinear method easy_transform_step(glinear b: Variables, ghost step: Step)
+//   returns (glinear c: Variables)
+//     requires TransitionEnable(b, step)
+//     ensures c == GetTransition(b, step)
+//   {
+//     var e := GetTransition(b, step);
+//     c := do_transform(b, e);
+//   }
 
-  predicate TransitionEnable(s: Variables, step: Step)
-  {
-    match step {
-    }
-  }
+//   lemma NewTicketPreservesValid(r: Variables, id: int, input: Ifc.Input)
+//     //requires Valid(r)
+//     ensures Valid(add(r, input_ticket(id, input)))
+//   {
+//     // reveal Valid();
+//     var ticket := input_ticket(id, input);
+//     var t :| Inv(add(r, t));
 
-  function GetTransition(s: Variables, step: Step): (s': Variables)
-    requires TransitionEnable(s, step)
-    ensures NextStep(s, s', step);
-  {
-    match step {
-    }
-  }
+//     assert add(add(r, ticket), t).table == add(r, t).table;
+//     assert add(add(r, ticket), t).insert_capacity == add(r, t).insert_capacity;
+//   }
 
-  // Reduce boilerplate by letting caller provide explicit step, which triggers a quantifier for generic Next()
-  glinear method easy_transform_step(glinear b: Variables, ghost step: Step)
-  returns (glinear c: Variables)
-    requires TransitionEnable(b, step)
-    ensures c == GetTransition(b, step)
-  {
-    var e := GetTransition(b, step);
-    c := do_transform(b, e);
-  }
+//   // Trusted composition tools. Not sure how to generate them.
+//   glinear method {:extern} enclose(glinear a: Count.Variables) returns (glinear h: Variables)
+//     requires Count.Valid(a)
+//     ensures h == unit().(insert_capacity := a)
 
-  lemma NewTicketPreservesValid(r: Variables, id: int, input: Ifc.Input)
-    //requires Valid(r)
-    ensures Valid(add(r, input_ticket(id, input)))
-  {
-    // reveal Valid();
-    var ticket := input_ticket(id, input);
-    var t :| Inv(add(r, t));
-
-    assert add(add(r, ticket), t).table == add(r, t).table;
-    assert add(add(r, ticket), t).insert_capacity == add(r, t).insert_capacity;
-  }
-
-  // Trusted composition tools. Not sure how to generate them.
-  glinear method {:extern} enclose(glinear a: Count.Variables) returns (glinear h: Variables)
-    requires Count.Valid(a)
-    ensures h == unit().(insert_capacity := a)
-
-  glinear method {:extern} declose(glinear h: Variables) returns (glinear a: Count.Variables)
-    requires h.Variables?
-    requires h.table == unitTable() // h is a unit() except for a
-    requires h.tickets == multiset{}
-    requires h.stubs == multiset{}
-    ensures a == h.insert_capacity
-*/  
+//   glinear method {:extern} declose(glinear h: Variables) returns (glinear a: Count.Variables)
+//     requires h.Variables?
+//     requires h.table == unitTable() // h is a unit() except for a
+//     requires h.tickets == multiset{}
+//     requires h.stubs == multiset{}
+//     ensures a == h.insert_capacity
+// */  
 }
